

Problems for the Calculus Tutorial

Ivan Savov, Minireference Co.

January 19, 2026

Limits

P1 Calculate the following limit expressions:

$$(a) \lim_{x \rightarrow \infty} \frac{7}{x+4} \quad (b) \lim_{x \rightarrow \infty} \frac{4x^2-7x+1}{x^2} \quad (c) \lim_{x \rightarrow 0^-} \frac{1}{x}$$

1 (a) 0. (b) 4. (c) $-\infty$.

1 a) As x goes to infinity, the denominator goes to infinity, so the fraction goes to zero.

b) If we divide each term by x^2 , we get the expression $\frac{4x^2-7x+1}{x^2} = 4 - \frac{7}{x} + \frac{1}{x^2}$. The limit of the first term is 4. The limits of the second and third terms are zero as x goes to infinity.

c) As x approaches 0 from the left ($x \rightarrow 0^-$), the fraction $\frac{1}{x}$ takes on larger and larger negative numbers. Therefore $\lim_{x \rightarrow 0^-} \frac{1}{x} = -\infty$.

P2 Assuming $\lim_{x \rightarrow \infty} f(x) = 2$ and $\lim_{x \rightarrow \infty} g(x) = 3$, compute

$$(a) \lim_{x \rightarrow \infty} (2f(x) - g(x)) \quad (b) \lim_{x \rightarrow \infty} f(x)g(x) \quad (c) \lim_{x \rightarrow \infty} \frac{4f(x)}{g(x) + 1}.$$

2 (a) 1. (b) 6. (c) 2.

2 We're given $\lim_{x \rightarrow \infty} f(x) = 2$ and $\lim_{x \rightarrow \infty} g(x) = 3$. For a) we use the sum rule:

$$\lim_{x \rightarrow \infty} (2f(x) - g(x)) = 2 \lim_{x \rightarrow \infty} f(x) - \lim_{x \rightarrow \infty} g(x) = 2 \cdot 2 - 3 = 1.$$

To solve b), we use the product rule for limits:

$$\lim_{x \rightarrow \infty} f(x)g(x) = \left(\lim_{x \rightarrow \infty} f(x) \right) \left(\lim_{x \rightarrow \infty} g(x) \right) = 2 \cdot 3 = 6.$$

To solve c) we use the quotient rule for limits:

$$\lim_{x \rightarrow \infty} \frac{4f(x)}{g(x) + 1} = \frac{4 \lim_{x \rightarrow \infty} f(x)}{\lim_{x \rightarrow \infty} (g(x) + 1)} = \frac{8}{\lim_{x \rightarrow \infty} g(x) + 1} = \frac{8}{3 + 1} = 2.$$

Derivatives

P3 Find the derivative with respect to x of the functions:

$$(a) f(x) = x^{13} \quad (b) g(x) = \sqrt[3]{x} \quad (c) h(x) = ax^2 + bx + c.$$

$$3 \quad f'(x) = 13x^{12}. \quad g'(x) = \frac{1}{3}x^{-\frac{2}{3}}. \quad h'(x) = 2ax + b.$$

$$3 \quad a) \text{ Use the power rule } \frac{d}{dx}x^n = nx^{n-1}: f'(x) = \frac{d}{dx}x^{13} = 13x^{12}.$$

$$b) \text{ Rewrite } \sqrt[3]{x} = x^{1/3} \text{ and use the power rule: } g'(x) = \frac{d}{dx}x^{1/3} = \frac{1}{3}x^{-2/3}.$$

$$c) \text{ Differentiate term-by-term: } h'(x) = \frac{d}{dx}(ax^2 + bx + c) = 2ax + b.$$

P4 Calculate the derivatives of the following functions:

$$(a) p(x) = \frac{2x+3}{3x+2} \quad (b) q(x) = \sqrt{x^2+1} \quad (c) r(\theta) = \sin^3 \theta.$$

$$4 \quad p'(x) = \frac{-5}{(3x+2)^2}. \quad q'(x) = \frac{x}{\sqrt{x^2+1}}. \quad r'(\theta) = 3\sin^2 \theta \cos \theta.$$

$$4 \quad a) \text{ Use the quotient rule } \left(\frac{u}{v}\right)' = \frac{u'v - uv'}{v^2} \text{ with } u = 2x+3 \text{ and } v = 3x+2:$$

$$p'(x) = \frac{2(3x+2) - (2x+3) \cdot 3}{(3x+2)^2} = \frac{6x+4-6x-9}{(3x+2)^2} = \frac{-5}{(3x+2)^2}.$$

$$b) \text{ Write } q(x) = (x^2+1)^{\frac{1}{2}} \text{ and use the chain rule:}$$

$$q'(x) = \frac{1}{2}(x^2+1)^{-\frac{1}{2}} \cdot 2x = \frac{x}{\sqrt{x^2+1}}.$$

$$c) \text{ Using the chain rule gives us } r'(\theta) = 3\sin^2 \theta \cdot \cos \theta.$$

P5 Find the maximum and the minimum of $f(x) = x^5 - 5x$.

$$5 \quad \text{Max at } x = -1; \text{ min at } x = 1.$$

5 First we compute the derivative $f'(x) = 5x^4 - 5 = 5(x^4 - 1)$. The critical points are $x = -1$ and $x = 1$. The second derivative is $f''(x) = 20x^3$. We apply the second derivative test to each critical point:

$$f''(-1) = -20 < 0 \Rightarrow \text{local maximum at } x = -1,$$

$$f''(1) = 20 > 0 \Rightarrow \text{local minimum at } x = 1.$$

Integrals

P6 Calculate the integral function $F_0(b) = \int_0^b f(x) dx$ for the polynomial $f(x) = 4x^3 + 3x^2 + 2x + 1$.

6 $F_0(b) = b^4 + b^3 + b^2 + b$.

6 Integrate term-by-term using the formula $\int_0^b x^n dx = \frac{1}{n+1} b^{n+1}$.

P7 Find the area under $f(x) = 8 - x^3$ between $x = 0$ and $x = 2$.

7 $A_f(0, 2) = 12$.

7 We compute the area using the definite integral:

$$A_f(0, 2) = \int_0^2 (8 - x^3) dx = \left[8x - \frac{x^4}{4} \right]_0^2 = \left(16 - \frac{16}{4} \right) - 0 = 12.$$

P8 Find the area under the graph of $g(x) = \sin(x)$ from $x = 0$ to $x = \pi$.

8 $A_g(0, \pi) = 2$.

8 The area is given by the following integral:

$$A_g(0, \pi) = \int_0^\pi \sin(x) dx = (-\cos \pi) - (-\cos 0) = 1 - (-1) = 2.$$

P9 Compute $\int_0^1 \frac{4x}{(1+x^2)^3} dx$ using the substitution $u = 1 + x^2$. Check your answer numerically using the SciPy function quad.

9 $\frac{3}{4}$.

9 When using the change of variable $u = 1 + x^2$, we must also change the differential $du = 2x dx$, which conveniently contains x that appears in the numerator, which allows us to write:

$$\int_{x=0}^{x=1} \frac{4x}{(1+x^2)^3} dx = \int_{x=0}^{x=1} \frac{2}{u^3} du = \int_{x=0}^{x=1} 2u^{-3} du.$$

Next we must change the x -limits of integration to u -limits of integration: The lower limit $x = 0$ becomes $u = 1 + 0^2 = 1$, and the upper limit $x = 1$ becomes $u = 1 + 1^2 = 2$, which the complete substitution:

$$\int_{x=0}^{x=1} \frac{4x}{(1+x^2)^3} dx = 2 \int_{u=1}^{u=2} u^{-3} du.$$

We can now proceed using the integral rule $\int x^n dx = \frac{1}{n+1} x^{n+1} + C$ to obtain

$$\begin{aligned} 2 \int_{u=1}^{u=2} u^{-3} du &= 2 \left[\frac{u^{-2}}{-2} \right]_1^2 = - \left[u^{-2} \right]_1^2 = - \left[\frac{1}{u^2} \right]_1^2 \\ &= - \left(\frac{1}{2^2} - \frac{1}{1^2} \right) = - \left(\frac{1}{4} - 1 \right) = \frac{3}{4} \end{aligned}$$

Sequences and series

P10 Calculate the value of the infinite series $\sum_{k=0}^{\infty} \left(\frac{2}{3}\right)^k$.

10 3.

10 We can use the formula for the geometric series $\sum_{k=0}^{\infty} r^k = \frac{1}{1-r}$ with $r = \frac{2}{3}$, which gives us $\sum_{k=0}^{\infty} \left(\frac{2}{3}\right)^k = \frac{1}{1-\frac{2}{3}} = 3$.

P11 Find the Taylor series for the function $f(x) = e^{-x}$.

Hint: Use algebraic manipulations starting from a Taylor series that you know.

11 $f(x) = \sum_{k=0}^{\infty} \frac{(-1)^k x^k}{k!}$.

11 Start from the known Taylor series $e^x = \sum_{k=0}^{\infty} \frac{x^k}{k!}$. Substitute $-x$ for x to get

$$f(x) = \sum_{k=0}^{\infty} \frac{(-x)^k}{k!} = \sum_{k=0}^{\infty} \frac{(-1)^k x^k}{k!}.$$

Answers

P1 (a) 0. (b) 4. (c) $-\infty$. **P2** (a) 1. (b) 6. (c) 2. **P3** $f'(x) = 13x^{12}$. $g'(x) = \frac{1}{3}x^{-\frac{2}{3}}$.
 $h'(x) = 2ax + b$. **P4** $p'(x) = \frac{-5}{(3x+2)^2}$. $q'(x) = \frac{x}{\sqrt{x^2+1}}$. $r'(\theta) = 3\sin^2\theta\cos\theta$. **P5**
Max at $x = -1$; min at $x = 1$. **P6** $F_0(b) = b^4 + b^3 + b^2 + b$. **P7** $A_f(0, 2) = 12$.
P8 $A_g(0, \pi) = 2$. **P9** $\frac{3}{4}$. **P10** 3. **P11** $f(x) = \sum_{k=0}^{\infty} \frac{(-1)^k x^k}{k!}$.